---
title: Review Session
date: 2017-12-06
categories: ELEC 321
use_math: true
---


- toc
{:toc}

## Problems

### Problem 1

Suppose we have $$Z_n=\frac{3}{4}Z_{n-1}+X_n$$ with $$Z_0=0$$ where $$X_n\sim \text{Bernoulli}$$

We can start by finding the Fourier transform of $$Z$$:

$$
Z(f)=\frac{3}{4}Z(f)e^{-j2\pi f}+X(f)
$$

Now factor out $$Z(f)$$ and find the $$H(f)$$:

$$
H(f)=\frac{1}{1-\frac{3}{4}e^{-j2\pi f}}
$$

We recognize that the signal in time domain is

$$
h(n)=(\frac{3}{4})^n u(n)
$$

Thus we know that the output has $$h(n)$$ convolved with the input (product in frequency domain)

$$
Z_n=h_n*X_n=\sum_{m=-\infty}^\infty X_m h_{n-m}=\sum_{m=1}^n X_m (\frac{3}{4})^{n-m}\\
=X_1(\frac34)^{n-1}+X_2(\frac34)^{n-2}+\dots+X_n
$$

**What is the expected value of $$Z_n$$?**

$$
\mathbb E(Z_n)=\mathbb E(X_1(\frac34)^{n-1})+\mathbb E(\dots)+\dots\\
=\mathbb E(X_1)(\frac34)^{n-1}+\mathbb E(X_2)(\frac34)^{n-2}+\dots\\
$$

Since $$\mathbb E(X_1)=\mathbb E(X_2)=\dots$$, then

$$
=\mathbb E(X)[1+\frac34+(\frac34)^2+\dots]\\
=\mathbb E(X)\frac{1-(\frac34)^n}{1-\frac34}
$$

Since the second term is a geometric series.

We see that as time $$n$$ increases, the mean of $$Z$$ is changing, thus $$Z$$ is not a stationary process.



### Problem 2

Packets arrive at probability $$a$$; packets depart at probability $$b$$. The buffer can hold up to $$N$$ packets. Let $$X_n$$ be the number of packets in the buffer at time $$n$$.

**Show that the system can be modelled by Markov Chain:**

Since at any time $$n$$ we don't care about the number of packets in the buffer at time $$n-2$$ (history) if we already have all the information $$n-1$$. In particular,

$$
\mathbb P(X_{n+1}=x_{n+1}\vert X_n=x_n, X_{n-1}=x_{n-1\dots})
$$

The conditional stuff (after that $$\vert $$ symbol) in the probability is useless information as far as the buffer is concerned.

There are total of $$N+1$$ states in the Markov chain: state $$\in\{0,1,\dots,n-1,n,n+1,\dots,N-1, N\}$$

For state 0: there are two possible states to go to:

- There is a $$1-a$$ probability that we will stay in state 0
- probability $$a$$ to go to state 1

For state $$N$$: there are also only two possible states to go

- $$1-b$$ probability that we stay in state $$N$$
- $$a$$ is the probability that we go to state $$N-1$$

For any state in between (state 1 to state $$N-1$$) there are three possible outcomes:

- probability of $$b(1-a)$$ of going to a lower state; since we need one packet to be transmitted and no packets arrive. The probabilities are $$b$$ and $$1-a$$ respectively. Since packet being received by the buffer and transmitted by the buffer is independent, the probability that $$X_n$$ goes from some number $$k$$ to $$k-1$$ is $$b(1-a)$$.
- probability of $$a(1-b)$$ of going to a higher state (same argument from above applies)
- probability of $$ab+(1-a)(1-b)$$ of staying in the same state. This occurs when (no packets are received $$\wedge$$ no packets are transmitted) $$\vee$$ (packet arrives $$\wedge$$ packet transmitted).

Therefore, the transition matrix is:

$$
P=\begin{bmatrix}
1-a & a & 0  & 0 & \cdots &0&0\\
b(1-a) & ab+(1-a)(1-b) & a(1-b) & 0 & \cdots &0&0\\
\vdots	& \ddots && &&& \vdots\\
0 &0&0&0&\cdots&b&1-b
\end{bmatrix}
$$

To find the **stationary distribution**, we use the fact that

$$
\pi=\pi P
$$

Do the matrix multiplication and we obtain $$N$$ equations for $$N$$ variables: $$\pi_1,\pi_2\dots, \pi_N$$.

The equations are:

$$
\begin{align}
\pi_0&=\pi_0(1-a)+\pi_1b(1-a)\\
\pi_1&=\pi_0(a)+\pi_1(ab+(1-a)(1-b))\dots\\
\vdots\\
\pi_N&=\dots
\end{align}
$$

Then we substitute every equation in terms of $$\pi_0$$, and for general $$n$$, we find the pattern:

$$
\pi_n=\frac{a^n(1-b)}{b^n(1-a)^n}\pi_0
$$

Then find $$\pi_0$$ by setting an initial condition.



## Office Hour

The variance for two normal random variables added together is the sum of two variances. (Proof later)















